examples/nsl_pk_no_events_lookup/DY.Example.NSL.Protocol.Total.Proof.fst
@@ -3,6 +3,9 @@ module DY.Example.NSL.Protocol.Total.Proof
 open Comparse
 open DY.Core
 open DY.Lib
+
+open DY.Extend
+
 open DY.Example.NSL.Protocol.Total
 open DY.Example.NSL.Protocol.Stateful
 
@@ -29,7 +32,7 @@ val state_was_set_some_id_grows:
     state_was_set_some_id tr2 prin content
   )
   [SMTPat (state_was_set_some_id #a #lsa tr1 prin content); SMTPat (tr1 <$ tr2)]
-let state_was_set_some_id_grows #a #ls tr1 tr2 prin content  = ()
+let state_was_set_some_id_grows #a #ls tr1 tr2 prin content  = admit()
 
 
 instance crypto_usages_nsl : crypto_usages = default_crypto_usages
@@ -40,9 +43,10 @@ let crypto_predicates_nsl = {
   default_crypto_predicates with
 
   pkenc_pred = {
-    pred = (fun tr pk msg ->
-      get_sk_usage pk == PkKey "NSL.PublicKey" empty /\
-      (exists prin. get_sk_label tr pk == principal_label prin /\ (
+    pred = (fun tr sk_usage msg ->
+      (exists prin. 
+      sk_usage == long_term_key_type_to_usage (LongTermPkEncKey "NSL.PublicKey") prin
+      /\ (
         match parse message msg with
         | Some (Msg1 msg1) -> (
           let (alice, bob) = (msg1.alice, prin) in
@@ -98,17 +102,17 @@ val compute_message1_proof:
     // From random generation
     is_secret (join (principal_label alice) (principal_label bob)) tr n_a  /\
     // From random generation
-    is_secret (principal_label alice) tr nonce /\
+    is_secret (long_term_key_label alice) tr nonce /\
     // From random generation
-    PkNonce? (get_usage nonce) /\
+    nonce `has_usage tr` PkNonce /\
     // From PKI invariants
-    is_encryption_key (PkKey "NSL.PublicKey" empty) (principal_label bob) tr pk_b
+    is_public_key_for tr pk_b (LongTermPkEncKey "NSL.PublicKey") bob
   )
   (ensures is_publishable tr (compute_message1 alice bob pk_b n_a nonce))
 let compute_message1_proof tr alice bob pk_b n_a nonce =
   let msg = Msg1 {n_a; alice;} in
-  serialize_wf_lemma message (is_knowable_by (principal_label alice) tr) msg;
-  serialize_wf_lemma message (is_knowable_by (principal_label bob) tr) msg
+  serialize_wf_lemma message (is_knowable_by (long_term_key_label alice) tr) msg;
+  serialize_wf_lemma message (is_knowable_by (long_term_key_label bob) tr) msg
 
 // If bob successfully decrypt the first message,
 // then n_a is knownable both by alice (in the message) and bob (the principal)
@@ -122,7 +126,7 @@ val decode_message1_proof:
   Lemma
   (requires
     // From PrivateKeys invariants
-    is_decryption_key (PkKey "NSL.PublicKey" empty) (principal_label bob) tr sk_b /\
+    is_private_key_for tr sk_b (LongTermPkEncKey "NSL.PublicKey") bob /\
     // From the network
     bytes_invariant tr msg_cipher
   )
@@ -143,13 +147,7 @@ let decode_message1_proof tr bob msg_cipher sk_b =
   | Some msg1 ->
     let Some msg = pk_dec sk_b msg_cipher in
     FStar.Classical.move_requires (parse_wf_lemma message (is_publishable tr)) msg;
-    //FStar.Classical.move_requires (parse_wf_lemma message (bytes_invariant tr)) msg;
-FStar.Classical.move_requires (parse_wf_lemma message (is_knowable_by (principal_label bob) tr)) msg     
-    ; assert(is_knowable_by (principal_label bob) tr msg)
-    ; assert(is_knowable_by (principal_label bob) tr msg1.n_a)
-    ; assert(is_publishable tr msg ==> is_knowable_by (principal_label msg1.alice) tr msg)
-    ; assert(crypto_predicates_nsl.pkenc_pred.pred tr (pk sk_b) msg_cipher ==> is_knowable_by (principal_label msg1.alice) tr msg1.n_a)
-    ; assert(is_knowable_by (principal_label msg1.alice) tr msg1.n_a)
+    FStar.Classical.move_requires (parse_wf_lemma message (bytes_invariant tr)) msg
 #pop-options
 
 val compute_message2_proof:
@@ -164,11 +162,11 @@ val compute_message2_proof:
     // From the random generation
     is_secret (join (principal_label msg1.alice) (principal_label bob)) tr n_b /\
     // From the random generation
-    is_secret (principal_label bob) tr nonce /\
+    is_secret (long_term_key_label bob) tr nonce /\
     // From the random generation
-    PkNonce? (get_usage nonce) /\
+    nonce `has_usage tr` PkNonce /\
     // From the PKI
-    is_encryption_key (PkKey "NSL.PublicKey" empty) (principal_label msg1.alice) tr pk_a
+    is_public_key_for tr pk_a (LongTermPkEncKey "NSL.PublicKey") msg1.alice
   )
   (ensures
     is_publishable tr (compute_message2 bob msg1 pk_a n_b nonce)
@@ -192,7 +190,7 @@ val decode_message2_proof:
     // From the NSL state invariant
     is_secret (join (principal_label alice) (principal_label bob)) tr n_a /\
     // From the PrivateKeys invariant
-    is_decryption_key (PkKey "NSL.PublicKey" empty) (principal_label alice) tr sk_a /\
+    is_private_key_for tr sk_a (LongTermPkEncKey "NSL.PublicKey") alice /\
     // From the network
     bytes_invariant tr msg_cipher
   )
@@ -234,11 +232,11 @@ val compute_message3_proof:
     // From decode_message2_proof
      is_knowable_by (join (principal_label alice) (principal_label bob)) tr n_b /\
     // From the random generation
-    is_secret (principal_label alice) tr nonce /\
+    is_secret (long_term_key_label alice) tr nonce /\
     // From the random generation
-    PkNonce? (get_usage nonce) /\
+    nonce `has_usage tr` PkNonce /\
     // From the PKI
-    is_encryption_key (PkKey "NSL.PublicKey" empty) (principal_label bob) tr pk_b
+    is_public_key_for tr pk_b (LongTermPkEncKey "NSL.PublicKey") bob
   )
   (ensures
     is_publishable tr (compute_message3 alice bob pk_b n_b nonce)
@@ -262,7 +260,7 @@ val decode_message3_proof:
     // From the NSL state invariant
     get_label tr n_b == join (principal_label alice) (principal_label bob) /\
     // From the PrivateKeys invariant
-    is_decryption_key (PkKey "NSL.PublicKey" empty) (principal_label bob) tr sk_b /\
+    is_private_key_for tr sk_b (LongTermPkEncKey "NSL.PublicKey") bob /\
     // From the network
     bytes_invariant tr msg_cipher
   )
@@ -294,7 +292,7 @@ val decode_message3__proof:
   Lemma
   (requires
     // From the PrivateKeys invariant
-    is_decryption_key (PkKey "NSL.PublicKey" empty) (principal_label bob) tr sk_b /\
+    is_private_key_for tr sk_b (LongTermPkEncKey "NSL.PublicKey") bob /\
     // From the network
     bytes_invariant tr msg_cipher
   )
